changed the calling convention to pass parameters on the stack (in particular load the parameter in the downwards lse example rather than dynamically check that it is below the stack bound), added some useful lemmas for world manipulation

theories/examples/macros/prepstack.v
@@ -39,35 +39,37 @@ Section stack_macros.
     { (* Failure, done *) by iApply "Hφ". }
   Qed.
 
-  Definition prepstackU_instrs r (minsize: Z) :=
+  Definition prepstackU_instrs r (minsize paramsize: nat) :=
     reqperm_instrs r (encodePerm URWLX) ++
-    reqsize_instrs r minsize ++
+    reqsize_instrs r (minsize + paramsize) ++
     [getb r_t1 r;
     geta r_t2 r;
+    sub_r_z r_t2 r_t2 paramsize;
     sub_r_r r_t1 r_t1 r_t2;
     lea_r r r_t1;
     move_z r_t1 0;
     move_z r_t2 0].
 
-  Definition prepstackU r minsize a p : iProp Σ :=
-    ([∗ list] a_i;w_i ∈ a;(prepstackU_instrs r minsize), a_i ↦ₐ[p] w_i)%I.
+  Definition prepstackU r minsize paramsize a p : iProp Σ :=
+    ([∗ list] a_i;w_i ∈ a;(prepstackU_instrs r minsize paramsize), a_i ↦ₐ[p] w_i)%I.
 
-  Lemma prepstackU_spec r minsize a w pc_p pc_p' pc_g pc_b pc_e a_first a_last φ :
+  Lemma prepstackU_spec r minsize paramsize a w pc_p pc_p' pc_g pc_b pc_e a_first a_last φ :
     isCorrectPC_range pc_p pc_g pc_b pc_e a_first a_last ->
     PermFlows pc_p pc_p' ->
     contiguous_between a a_first a_last ->
 
-      ▷ prepstackU r minsize a pc_p'
+      ▷ prepstackU r minsize paramsize a pc_p'
     ∗ ▷ PC ↦ᵣ inr (pc_p,pc_g,pc_b,pc_e,a_first)
     ∗ ▷ r ↦ᵣ w
     ∗ ▷ (∃ w, r_t1 ↦ᵣ w)
     ∗ ▷ (∃ w, r_t2 ↦ᵣ w)
     ∗ ▷ (if isPermWord w URWLX then
            ∃ l b e a', ⌜w = inr (URWLX,l,b,e,a')⌝ ∧
-           if (minsize <? e - b)%Z then
-             if (b <=? a')%Z then
-               (PC ↦ᵣ inr (pc_p,pc_g,pc_b,pc_e,a_last) ∗ prepstackU r minsize a pc_p' ∗
-                   r ↦ᵣ inr (URWLX,l,b,e,b) ∗ r_t1 ↦ᵣ inl 0%Z ∗ r_t2 ↦ᵣ inl 0%Z
+           if (minsize + paramsize <? e - b)%Z then
+             if ((b + paramsize) <=? a')%Z then
+               ((∃ a_param, ⌜(b + paramsize)%a = Some a_param⌝ ∧
+                   PC ↦ᵣ inr (pc_p,pc_g,pc_b,pc_e,a_last) ∗ prepstackU r minsize paramsize a pc_p' ∗
+                   r ↦ᵣ inr (URWLX,l,b,e,a_param) ∗ r_t1 ↦ᵣ inl 0%Z ∗ r_t2 ↦ᵣ inl 0%Z)
                    -∗ WP Seq (Instr Executable) {{ φ }})
              else φ FailedV
            else φ FailedV
@@ -90,7 +92,7 @@ Section stack_macros.
     iPrologue_multi "Hprog" Hcont Hvpc link0.
     iApply (reqsize_spec with "[- $HPC $Hcode $Hr $Hr_t1 $Hr_t2]");
       [apply Hvpc_code0|apply Hfl|eauto|].
-    iNext. destruct (minsize <? e - b)%Z; auto.
+    iNext. destruct (minsize + paramsize <? e - b)%Z eqn:Hsize; auto.
     iIntros "H". iDestruct "H" as (w1 w2) "(Hreqsize & HPC & Hr & Hr_t1 & Hr_t2)".
     (* getb r_t1 r *)
     iDestruct (big_sepL2_length with "Hprog") as %Hlength'.
@@ -98,46 +100,53 @@ Section stack_macros.
     iPrologue "Hprog".
     iApply (wp_Get_success with "[$HPC $Hi $Hr $Hr_t1]");
       [apply decode_encode_instrW_inv|auto|apply Hfl|iCorrectPC link0 a_last|iContiguous_next Hcont 0|auto..].
-    iEpilogue "(HPC & Hi & Hr & Hr_t1) /="; iCombine "Hi" "Hprog_done" as "Hprog_done". 
+    iEpilogue "(HPC & Hi & Hr & Hr_t1) /="; iCombine "Hi" "Hprog_done" as "Hprog_done".
     (* geta r_t2 r *)
     iPrologue "Hprog".
     iApply (wp_Get_success with "[$HPC $Hi $Hr $Hr_t2]");
       [apply decode_encode_instrW_inv|auto|apply Hfl|iCorrectPC link0 a_last|iContiguous_next Hcont 1|auto..].
-    iEpilogue "(HPC & Hi & Hr & Hr_t2) /="; iCombine "Hi" "Hprog_done" as "Hprog_done". 
+    iEpilogue "(HPC & Hi & Hr & Hr_t2) /="; iCombine "Hi" "Hprog_done" as "Hprog_done".
+    (* add r_t2 r_t2 paramsize *)
+    iPrologue "Hprog".
+    iApply (wp_add_sub_lt_success_dst_z with "[$HPC $Hi $Hr_t2]");
+      [apply decode_encode_instrW_inv|auto|iContiguous_next Hcont 2|apply Hfl|iCorrectPC link0 a_last|..].
+    iEpilogue "(HPC & Hi & Hr_t2) /="; iCombine "Hi" "Hprog_done" as "Hprog_done".
     (* sub r_t1 r_t1 r_t2 *)
     iPrologue "Hprog".
     iApply (wp_add_sub_lt_success_dst_r with "[$HPC $Hi $Hr_t2 $Hr_t1]");
-      [apply decode_encode_instrW_inv|auto|iContiguous_next Hcont 2|apply Hfl|iCorrectPC link0 a_last|..].
+      [apply decode_encode_instrW_inv|auto|iContiguous_next Hcont 3|apply Hfl|iCorrectPC link0 a_last|..].
     iEpilogue "(HPC & Hi & Hr_t2 & Hr_t1) /="; iCombine "Hi" "Hprog_done" as "Hprog_done".
     (* we need to distinguish between the case where the capability is stuck, or usable *)
-    assert ((a' + (b - a'))%a = Some b) as Hlea;[solve_addr|].
-    destruct (decide (b <= a')%a).
+    assert (∃ a_param, (b + paramsize)%a = Some a_param) as [a_param Ha_param].
+    { destruct (b + paramsize)%a eqn:Hnone;eauto. exfalso. clear -Hnone Hsize. apply Z.ltb_lt in Hsize. solve_addr. }
+    assert ((a' + (b - (a' - paramsize)))%a = Some a_param) as Hlea;[clear -Ha_param; solve_addr|].
+    destruct (decide (a_param <= a')%a).
     2: { (* lea fail *)
       iPrologue "Hprog".
       iApply (wp_Lea_fail_U with "[$HPC $Hi $Hr_t1 $Hr]");
         [apply decode_encode_instrW_inv|apply Hfl|iCorrectPC link0 a_last|apply Hlea|..].
       { simpl. solve_addr. }
-      iEpilogue "_ /=". assert (b <=? a' = false)%Z as ->;[apply Z.leb_gt;solve_addr|].
+      iEpilogue "_ /=". assert (b + paramsize <=? a' = false)%Z as ->;[apply Z.leb_gt;solve_addr|].
       iApply wp_value. iApply "Hφ". }
     (* lea r r_t1 *)
     iPrologue "Hprog".
     iApply (wp_lea_success_reg with "[$HPC $Hi $Hr_t1 $Hr]");
-      [apply decode_encode_instrW_inv|apply Hfl|iCorrectPC link0 a_last|iContiguous_next Hcont 3|apply Hlea|auto..].
-    iEpilogue "(HPC & Hi & Hr_t1 & Hr)"; iCombine "Hi" "Hprog_done" as "Hprog_done". 
+      [apply decode_encode_instrW_inv|apply Hfl|iCorrectPC link0 a_last|iContiguous_next Hcont 4|apply Hlea|auto..].
+    iEpilogue "(HPC & Hi & Hr_t1 & Hr)"; iCombine "Hi" "Hprog_done" as "Hprog_done".
     (* move r_t1 0 *)
     iPrologue "Hprog".
-    iApply (wp_move_success_z with "[$HPC $Hi $Hr_t1]"); 
-      [apply decode_encode_instrW_inv|apply Hfl|iCorrectPC link0 a_last|iContiguous_next Hcont 4|auto|..].
-    iEpilogue "(HPC & Hi & Hr_t1)"; iCombine "Hi" "Hprog_done" as "Hprog_done". 
+    iApply (wp_move_success_z with "[$HPC $Hi $Hr_t1]");
+      [apply decode_encode_instrW_inv|apply Hfl|iCorrectPC link0 a_last|iContiguous_next Hcont 5|auto|..].
+    iEpilogue "(HPC & Hi & Hr_t1)"; iCombine "Hi" "Hprog_done" as "Hprog_done".
     (* move r_t2 0 *)
     iPrologue "Hprog".
-    apply contiguous_between_last with (ai:=a4) in Hcont as Hlast;[|auto].
-    iApply (wp_move_success_z with "[$HPC $Hi $Hr_t2]"); 
+    apply contiguous_between_last with (ai:=a5) in Hcont as Hlast;[|auto].
+    iApply (wp_move_success_z with "[$HPC $Hi $Hr_t2]");
       [apply decode_encode_instrW_inv|apply Hfl|iCorrectPC link0 a_last|apply Hlast|auto|..].
-    iEpilogue "(HPC & Hi & Hr_t2)"; iCombine "Hi" "Hprog_done" as "Hprog_done". 
-    assert (b <=? a' = true)%Z as ->;[apply Zle_is_le_bool;auto|].
-    iApply "Hφ". iFrame.
-    repeat (iDestruct "Hprog_done" as "[Hi Hprog_done]"; iFrame "Hi"). 
+    iEpilogue "(HPC & Hi & Hr_t2)"; iCombine "Hi" "Hprog_done" as "Hprog_done".
+    assert (b + paramsize <=? a' = true)%Z as ->;[apply Zle_is_le_bool;auto;clear -Ha_param l0;solve_addr|].
+    iApply "Hφ". iFrame. iExists a_param. iSplit;auto. iFrame.
+    repeat (iDestruct "Hprog_done" as "[Hi Hprog_done]"; iFrame "Hi").
     iFrame "Hprog_done". done.
   Qed.
 
