theories/examples/downwards_lse.v
@@ -17,9 +17,9 @@ Section lse.
 
 
   Definition lse_instrs f_a :=
-    prepstackU_instrs r_stk 1 ++
-    checkbelow_instrs r_t0 r_stk ++
-    [pushU_r_instr r_stk r_env;
+    prepstackU_instrs r_stk 1 1 ++
+    [loadU_r_z r_t0 r_stk (-1); (* since parameters are passer on the stack, no need to check that the input is below the stack bound *)
+    pushU_r_instr r_stk r_env;
     load_r r_env r_env] ++
     assert_r_z_instrs f_a r_env 2 ++
     rclear_instrs (list_difference all_registers [PC;r_t0]) ++
@@ -32,7 +32,6 @@ Section lse.
 
 
   Lemma lse_spec W pc_p pc_p' pc_g pc_b pc_e (* PC *)
-        wret (* return cap *)
         lse_addrs (* program addresses *)
         d d' (* dynamically allocated memory given by preamble, connected to invariant i *)
         a_first a_last (* special adresses *)
@@ -56,14 +55,13 @@ Section lse.
     (d + 1)%a = Some d' ->
 
     (* footprint of the register map *)
-    dom (gset RegName) rmap = all_registers_s ∖ {[PC;r_stk;r_t0;r_env]} →
+    dom (gset RegName) rmap = all_registers_s ∖ {[PC;r_stk;r_env]} →
 
     (* The two invariants have different names *)
     (up_close (B:=coPset) ι2 ## ↑ι1) ->
 
     {{{ r_stk ↦ᵣ wstk
       ∗ PC ↦ᵣ inr ((pc_p,pc_g),pc_b,pc_e,a_first)
-      ∗ r_t0 ↦ᵣ wret
       ∗ r_env ↦ᵣ inr (RWX,Global,d,d',d)
       ∗ ([∗ map] r_i↦w_i ∈ rmap, r_i ↦ᵣ w_i)
       (* invariant for d *)
@@ -72,8 +70,6 @@ Section lse.
       ∗ interp W wstk
       (* token which states all non atomic invariants are closed *)
       ∗ na_own logrel_nais ⊤
-      (* callback validity *)
-      ∗ interp W wret
       (* trusted code *)
       ∗ na_inv logrel_nais ι1 (lse lse_addrs pc_p' f_a)
       (* linking table *)
@@ -91,15 +87,17 @@ Section lse.
                          ∗ region W' }}}.
   Proof.
     iIntros (Hvpc Hfl Hcont Hlt_wb Hlt_link Hdoff Hdom Hndisj φ).
-    iIntros "(Hr_stk & HPC & Hr_t0 & Hr_env & Hregs & #Hdinv & #Hwstk_valid & Hown & #Hwret_valid & #Hlse_prog & #Htable & Hsts & Hr) Hφ".
+    iIntros "(Hr_stk & HPC & Hr_env & Hregs & #Hdinv & #Hwstk_valid & Hown & #Hlse_prog & #Htable & Hsts & Hr) Hφ".
     iMod (na_inv_acc with "Hlse_prog Hown") as "(>Hprog & Hown & Hcls)";auto.
     (* get some general purpose registers *)
+    assert (is_Some (rmap !! r_t0)) as [w0 Hw0];[apply elem_of_gmap_dom;rewrite Hdom;set_solver+|].
     assert (is_Some (rmap !! r_t1)) as [w1 Hw1];[apply elem_of_gmap_dom;rewrite Hdom;set_solver+|].
     assert (is_Some (rmap !! r_t2)) as [w2 Hw2];[apply elem_of_gmap_dom;rewrite Hdom;set_solver+|].
     assert (is_Some (rmap !! r_t3)) as [w3 Hw3];[apply elem_of_gmap_dom;rewrite Hdom;set_solver+|].
     assert (is_Some (rmap !! r_t4)) as [w4 Hw4];[apply elem_of_gmap_dom;rewrite Hdom;set_solver+|].
-    iDestruct (big_sepM_delete with "Hregs") as "[Hr_t1 Hregs]";[apply Hw1|].
-    iDestruct (big_sepM_delete _ _ r_t2 with "Hregs") as "[Hr_t2 Hregs]";[rewrite lookup_delete_ne//;eauto|].
+    iDestruct (big_sepM_delete with "Hregs") as "[Hr_t0 Hregs]";[apply Hw0|].
+    iDestruct (big_sepM_delete _ _ r_t1 with "Hregs") as "[Hr_t1 Hregs]";[rewrite lookup_delete_ne//;eauto|].
+    iDestruct (big_sepM_delete _ _ r_t2 with "Hregs") as "[Hr_t2 Hregs]";[rewrite !lookup_delete_ne//;eauto|].
     iDestruct (big_sepM_delete _ _ r_t3 with "Hregs") as "[Hr_t3 Hregs]";[rewrite !lookup_delete_ne//;eauto|].
     iDestruct (big_sepM_delete _ _ r_t4 with "Hregs") as "[Hr_t4 Hregs]";[rewrite !lookup_delete_ne//;eauto|].
     (* prepstack *)
@@ -110,18 +108,31 @@ Section lse.
     (* cleanup of stack information *)
     destruct wstk as [| [ [ [ [p_stk l_stk] b_stk] e_stk] a_stk] ];[inversion Hperm|]. iExists l_stk,b_stk, e_stk, a_stk.
     destruct p_stk;inversion Hperm. iSplit;auto.
-    destruct (1 <? e_stk - b_stk)%Z eqn:Hsize;[|(* Failure *) iApply "Hφ";iIntros (Hcontr);inversion Hcontr].
-    destruct (b_stk <=? a_stk)%Z eqn:Hle;[|(* Failure *) iApply "Hφ";iIntros (Hcontr);inversion Hcontr].
+    destruct (1%nat + 1%nat <? e_stk - b_stk)%Z eqn:Hsize;[|(* Failure *) iApply "Hφ";iIntros (Hcontr);inversion Hcontr].
+    destruct (b_stk + 1%nat <=? a_stk)%Z eqn:Hle;[|(* Failure *) iApply "Hφ";iIntros (Hcontr);inversion Hcontr].
     iDestruct (writeLocalAllowedU_implies_local with "Hwstk_valid") as %Hmonotone;auto. destruct l_stk;inversion Hmonotone.
-    iIntros "(HPC & Hprepstack & Hr_stk & Hr_t1 & Hr_t2)".
-    (* checkbelow *)
+    iIntros "Hstack".
+    iDestruct "Hstack" as (a Ha) "(HPC & Hprepstack & Hr_stk & Hr_t1 & Hr_t2)".
+    apply Z.leb_le in Hle. apply Z.ltb_lt in Hsize.
+    (* pop r_stk r_t0 *)
+    (* in order to pop, we must first open the region at b_stk *)
+    iDestruct (writeLocalAllowedU_valid_cap_below_implies _ _ _ _ _ _ b_stk with "Hwstk_valid") as %Ha_param_W;[auto|..].
+    { clear -Hle Hsize Ha. rewrite andb_true_iff Z.leb_le Z.ltb_lt. solve_addr. }
+    { clear -Hle;solve_addr. }
+    iDestruct (read_allowedU_inv _ b_stk with "Hwstk_valid") as (p' Hfl') "Hrel";[clear -Hsize;solve_addr|auto|]. destruct p'; inversion Hfl'.
+    iDestruct (region_open_monotemp_pwl with "[$Hr $Hsts $Hrel]") as (wret) "(Hr & Hsts & Hstate & Hb_stk & % & #Hmono & #Hwret_valid)";auto.
+    iSimpl in "Hwret_valid".
+    (* loadU r_t0 r_stk -1 *)
     iPrologue_multi "Hprog" Hcont Hvpc link0.
-    iApply (checkbelow_spec with "[- $HPC $Hcode $Hr_stk $Hr_t0]");[eauto..|].
-    iSplitL "Hr_t1";[eauto|]. iSplitL "Hr_t2";[eauto|]. iSplitL "Hr_t3";[eauto|]. iSplitL "Hr_t4";[eauto|].
-    iNext.
-    destruct (is_cap wret && (canReadUpTo wret <? b_stk)%a && negb (isO_word wret)) eqn:Hbelowcond;
-      [|(* Failure *) iApply "Hφ";iIntros (Hcontr);inversion Hcontr].
-    iIntros "(HPC & Hcheckbelow & Hr_t0 & Hr_stk & Hr_t1 & Hr_t2 & Hr_t3 & Hr_t4)".
+    iDestruct (big_sepL2_length with "Hcode") as %Hlength1. destruct_addr_list l_code0.
+    iPrologue "Hcode". apply contiguous_between_cons_inv_first in Hcont_code0 as Heq. subst link.
+    iApply (rules_LoadU_derived.wp_loadU_success with "[$HPC $Hi $Hr_t0 $Hr_stk $Hb_stk]");
+      [apply decode_encode_instrW_inv|apply Hfl|auto|iCorrectPC l_code0 link0|auto..].
+    { clear -Hle Hsize Ha. rewrite andb_true_iff Z.leb_le Z.ltb_lt. solve_addr. }
+    { iContiguous_next_a Hcont_code0. }
+    iEpilogue "(HPC & Hr_t0 & Hprog_done & Hr_stk & Hb_stk)".
+    (* we can close the world again *)
+    iDestruct (region_close_monotemp_pwl with "[$Hstate $Hb_stk $Hr $Hrel $Hmono $Hwret_valid]") as "Hr";auto.
 
     (* pushu r_stk r_env *)
     (* we have reached a part of the code which will require us to make a pub^b_stk change to the world *)
@@ -129,51 +140,40 @@ Section lse.
     iMod (uninitialize_region _ b_stk with "[$Hsts $Hr]") as (m Hmcond) "[Hsts Hr]".
     (* next we can open the region at b_stk, which we will first assert is in m *)
     iDestruct (valid_uninitialized_condition _ m with "Hwstk_valid") as %Hstk_cond;auto.
-    (* next we can open the world at b_stk *)
-    assert (b_stk <= b_stk < e_stk)%a as Hstk_bounds.
-    { split;[clear;solve_addr|]. clear -Hsize. apply Z.ltb_lt in Hsize. lia. }
-    pose proof (Hstk_cond b_stk Hstk_bounds) as [w Hw].
-    iAssert (rel b_stk RWLX (λ Wv, interp Wv.1 Wv.2)) as "#Hrel".
-    { rewrite fixpoint_interp1_eq /=. destruct (decide (b_stk < a_stk))%a.
-      - iDestruct "Hwstk_valid" as "[Hv _]".
-        iDestruct (big_sepL_elem_of _ _ b_stk with "Hv") as (p Hflp) "[Hrel _]".
-        { apply elem_of_region_addrs. clear -Hstk_bounds l. solve_addr. }
-        destruct p;inversion Hflp. iFrame "Hrel".
-      - iDestruct "Hwstk_valid" as "[_ Hv]".
-        iDestruct (big_sepL_elem_of _ _ b_stk with "Hv") as (p Hflp) "[Hrel _]".
-        { apply elem_of_region_addrs. clear -Hstk_bounds n. solve_addr. }
-        destruct p;inversion Hflp. iFrame "Hrel". }
-    iDestruct (region_open_uninitialized with "[$Hrel $Hr $Hsts]") as "(Hr & Hsts & Hstate & Hb_stk & %)";[eauto|..].
+    (* next we can open the world at a *)
+    assert (b_stk <= a < e_stk)%a as Hstk_bounds.
+    { split;[clear -Ha;solve_addr|]. clear -Hsize Ha. solve_addr. }
+    pose proof (Hstk_cond a Hstk_bounds) as [w Hw]. clear Hfl'.
+    iDestruct (read_allowedU_inv _ a with "Hwstk_valid") as (p' Hfl') "Hrel'";[clear -Hsize Ha;solve_addr|auto|]. destruct p'; inversion Hfl'.
+    iDestruct (region_open_uninitialized with "[$Hrel' $Hr $Hsts]") as "(Hr & Hsts & Hstate & Ha & %)";[eauto|..].
     (* and we are ready to push a new value b_stk *)
-    assert (is_Some (b_stk + 1))%a as [b_stk1 Hb_next].
-    { clear -Hstk_bounds. destruct (b_stk + 1)%a eqn:Hsome;eauto. exfalso. solve_addr. }
-    iPrologue_multi "Hprog" Hcont Hvpc link1.
-    iDestruct (big_sepL2_length with "Hcode") as %Hlength_code1.
-    prep_addr_list_full l_code1 Hcont_code1.
+    assert (is_Some (a + 1))%a as [b_stk1 Hb_next].
+    { clear -Hstk_bounds. destruct (a + 1)%a eqn:Hsome;eauto. exfalso. solve_addr. }
     iDestruct "Hcode" as "[HpushU Hcode]".
-    iApply (pushU_r_spec with "[- $HPC $HpushU $Hr_stk $Hr_env $Hb_stk]");
-      [iCorrectPC link0 link1|auto|auto| |iContiguous_next_a Hcont_code1|apply Hb_next|..].
+    iApply (pushU_r_spec with "[- $HPC $HpushU $Hr_stk $Hr_env $Ha]");
+      [iCorrectPC l_code0 link0|auto|auto| |iContiguous_next_a Hcont_code0|apply Hb_next|..].
     { apply andb_true_iff. split;[apply Z.leb_le|apply Z.ltb_lt];clear -Hstk_bounds;solve_addr. }
     { intros Hcontr;inversion Hcontr. }
     iNext. iIntros "(HPC & HpushU & Hr_stk & Hr_env & Hb_stk)".
     (* we can now close the world again *)
     pose proof (uninitialized_condition _ _ _ Hmcond) as Hmcond_alt.
-    iMod (uninitialize_open_region_change _ _ b_stk with "[$Hb_stk $Hrel $Hsts $Hr $Hstate]") as "[Hr Hsts]";
+    iMod (uninitialize_open_region_change _ _ a with "[$Hb_stk $Hrel' $Hsts $Hr $Hstate]") as "[Hr Hsts]";
       [clear;solve_addr|auto|auto|].
+    { intros. apply Hmcond_alt. clear -H2 Ha. solve_addr. }
 
     (* and we can now finish executing the instructions without more changes to W *)
     iPrologue "Hcode".
     iDestruct "Hdinv" as (ι) "Hdinv". iInv ι as ">Hd" "Hcls'". rewrite /lse_inv.
-    iAssert (⌜(d =? a)%a = false⌝)%I as %Heq_false.
+    iAssert (⌜(d =? a1)%a = false⌝)%I as %Heq_false.
     { rewrite Z.eqb_neq. iIntros (->%z_of_eq). iDestruct (address_dupl_false with "Hi Hd") as "Hbot";[auto..|done].
-      eapply pc_range_nonO in Hcont_code1;[|eauto]. destruct pc_p',pc_p;auto;inversion Hfl;auto. }
+      eapply pc_range_nonO in Hcont_code0;[|eauto]. destruct pc_p',pc_p;auto;inversion Hfl;auto. }
     iApply (wp_load_success_same with "[$HPC $Hi $Hr_env Hd]");
-      [auto|apply decode_encode_instrW_inv|apply Hfl|iCorrectPC link0 link1|..].
+      [auto|apply decode_encode_instrW_inv|apply Hfl|iCorrectPC l_code0 link0|..].
     { clear -Hdoff. split;auto. apply andb_true_iff. split;[apply Z.leb_le|apply Z.ltb_lt];solve_addr. }
-    { eapply contiguous_between_last. apply Hcont_code1. auto. }
+    { eapply contiguous_between_last. apply Hcont_code0. auto. }
     { rewrite Heq_false. iFrame. auto. }
     rewrite Heq_false.
-    iNext. iIntros "(HPC & Hr_env & Hprog_done & Hd)".
+    iNext. iIntros "(HPC & Hr_env & Hi & Hd)". iCombine "Hi" "Hprog_done" as "Hprog_done".
     iMod ("Hcls'" with "[$Hd]") as "_".
     iModIntro. iApply wp_pure_step_later;auto. iNext.
     iClear "Hcode".
@@ -182,7 +182,7 @@ Section lse.
     iPrologue_multi "Hprog" Hcont Hvpc link2.
     iMod (na_inv_acc with "Htable Hown") as "(>[Hpc_b Ha_entry] & Hown & Hcls'')";[auto|solve_ndisj|].
     iApply (assert_r_z_success with "[- $HPC $Hcode $Hr_env $Hpc_b $Ha_entry]");
-      [apply Hvpc_code2|apply Hfl|apply Hcont_code2|auto..|].
+      [apply Hvpc_code1|apply Hfl|apply Hcont_code1|auto..|].
     iSplitL "Hr_t1";[eauto|]. iSplitL "Hr_t2";[eauto|]. iSplitL "Hr_t3";[eauto|].
     iNext. iIntros "(Hr_t1 & Hr_t2 & Hr_t3 & Hr_env & HPC & Hassert & Hpc_b & Ha_entry)".
     iMod ("Hcls''" with "[$Hown $Hpc_b $Ha_entry]") as "Hown".
@@ -194,57 +194,50 @@ Section lse.
     iDestruct (big_sepM_insert with "[$Hregs $Hr_t2]") as "Hregs";[apply lookup_delete|rewrite insert_delete -!delete_insert_ne//].
     iDestruct (big_sepM_insert with "[$Hregs $Hr_t1]") as "Hregs";[apply lookup_delete|rewrite insert_delete].
     iDestruct (big_sepM_insert with "[$Hregs $Hr_stk]") as "Hregs".
-    { rewrite !lookup_insert_ne//. apply not_elem_of_dom. rewrite Hdom. set_solver-. }
+    { rewrite lookup_insert_ne// lookup_delete_ne// !lookup_insert_ne//. apply not_elem_of_dom. rewrite Hdom. set_solver-. }
     iDestruct (big_sepM_insert with "[$Hregs $Hr_env]") as "Hregs".
-    { rewrite !lookup_insert_ne//. apply not_elem_of_dom. rewrite Hdom. set_solver-. }
+    { simplify_map_eq. apply not_elem_of_dom. rewrite Hdom. set_solver-. }
     iApply (rclear_spec_gmap with "[- $HPC $Hcode $Hregs]");[eauto..|].
     { apply not_elem_of_list. constructor. }
     { assert (length l_code2 = 31) as Hlength4. clear -Hlength2 Hlength3. rewrite app_length Hlength3 in Hlength2. lia.
-      destruct l_code2;inversion Hlength4. apply contiguous_between_cons_inv_first in Hcont_code3 as ->. auto. }
-    { clear -Hdom. rewrite !dom_insert_L Hdom list_to_set_difference -/all_registers_s /=. clear. set_solver. }
+      destruct l_code2;inversion Hlength4. apply contiguous_between_cons_inv_first in Hcont_code2 as ->. auto. }
+    { clear -Hdom. rewrite !dom_insert_L !dom_delete_L !dom_insert_L Hdom list_to_set_difference -/all_registers_s /=. clear. set_solver. }
     iNext. iIntros "[HPC [Hdom Hrclear]]".
     iDestruct "Hdom" as (rmap') "[Hregs #Hregs_cond]". iDestruct "Hregs_cond" as %[Hdom' Hzeroes].
 
     (* jmp r_t0 *)
-    prep_addr_list_full l_rest3 Hcont.
+    prep_addr_list_full l_rest2 Hcont.
     iPrologue "Hprog".
     iApply (wp_jmp_success with "[$HPC $Hi $Hr_t0]");
       [apply decode_encode_instrW_inv|apply Hfl|iCorrectPC link3 a_last|].
 
     (* first we will update the varilidy of wret to the new world *)
-    (* this will be possible because we made sure its reading bound is below b_stk *)
-    set (W' := (<s[b_stk:=Uninitialized (inr (RWX, Global, d, d', d))]s>(uninitialize W m))).
-    apply andb_true_iff in Hbelowcond as [ [His_cap Hlt%Z.ltb_lt]%andb_true_iff HnotO].
+    set (W' := (<s[a:=Uninitialized (inr (RWX, Global, d, d', d))]s>(uninitialize W m))).
     assert (related_sts_a_world W W' b_stk) as Hrelated.
     { eapply related_sts_a_trans_world;[apply uninitialize_related_pub_a|];eauto.
-      apply related_sts_a_uninitialized. clear -Hmcond Hmcond_alt His_cap Hlt HnotO Hw. solve_addr. eauto. }
-    iDestruct (interp_monotone_a _ W' with "[] Hwret_valid") as "Hwret_valid'".
-    { iPureIntro. clear -Hmcond Hmcond_alt His_cap Hlt HnotO Hw Hrelated. eapply related_sts_a_weak_world with b_stk;auto.
-      destruct wret;inversion His_cap. destruct c,p,p,p. simpl in *.
-      destruct (isU p) eqn:HU;destruct p;inversion Hlt;solve_addr. }
-    destruct wret;inversion His_cap. destruct c as [ [ [ [p g]b]e]a'].
-    iAssert (▷ interp_expression (<[PC:=inl 0%Z]> (<[r_t0:=inr (p, g, b, e, a')]> rmap')) W' (updatePcPerm (inr (p,g,b,e,a'))))%I as "Hcont".
-    { destruct (decide (p = E)).
-      - subst. iClear "Hwstk_valid Hwret_valid". rewrite fixpoint_interp1_eq. iSimpl in "Hwret_valid'".
-        rewrite /enter_cond. iApply "Hwret_valid'". destruct g;iPureIntro.
-        apply related_sts_priv_refl_world. apply related_sts_priv_refl_world. apply related_sts_a_refl_world.
-      - iDestruct (fundamental_from_interp (<[PC:=inl 0%Z]> (<[r_t0:=inr (p,g,b,e,a')]> rmap')) with "Hwret_valid'") as "Hcont". iNext.
-        rewrite updatePcPerm_cap_non_E//. }
+      apply related_sts_a_uninitialized. clear -Ha; solve_addr. apply Hstk_cond. auto. }
+    iDestruct ("Hmono" $! _ _ Hrelated with "Hwret_valid") as "Hwret_valid'". iSimpl in "Hwret_valid'".
+    iDestruct (jmp_or_fail_spec with "Hwret_valid'") as "Hcond". destruct (decide (isCorrectPC (updatePcPerm wret))).
+    2: { iEpilogue "(HPC & _)". iApply "Hcond". iFrame. iApply "Hφ". iIntros (Hcontr). inversion Hcontr. }
+    iDestruct "Hcond" as (p g b e a' Heq) "Hcond". rewrite Heq.
+    iSpecialize ("Hcond" $! (<[PC:=inl 0%Z]> (<[r_t0:=wret]> rmap')) W' with "[]").
+    { destruct g;iPureIntro.
+      apply related_sts_priv_refl_world. apply related_sts_priv_refl_world. apply related_sts_a_refl_world. }
 
     (* we can now establish the continuation *)
     iEpilogue "(HPC & Hi & Hr_t0)".
 
     (* first we will close the program invariant *)
-    iMod ("Hcls" with "[Hprepstack Hcheckbelow HpushU Hprog_done Hassert Hrclear Hi $Hown]") as "Hown".
-    { iNext. iFrame. simpl. done. }
+    iMod ("Hcls" with "[Hprepstack HpushU Hprog_done Hassert Hrclear Hi $Hown]") as "Hown".
+    { iNext. iFrame. iDestruct "Hprog_done" as "($&$)". simpl. done. }
 
     (* next we must establish that the current register state is valid *)
     iDestruct (big_sepM_insert with "[$Hregs $Hr_t0]") as "Hregs".
     { apply not_elem_of_dom. rewrite Hdom'. set_solver-. }
     iDestruct (big_sepM_insert with "[$Hregs $HPC]") as "Hregs".
     { rewrite lookup_insert_ne//. apply not_elem_of_dom. rewrite Hdom'. set_solver-. }
-    iDestruct ("Hcont" with "[$Hown $Hr $Hsts Hregs]") as "[_ Hconf]".
-    { rewrite insert_insert. iFrame "Hregs". iSplit;[iPureIntro|].
+    iDestruct ("Hcond" with "[$Hown $Hr $Hsts Hregs]") as "[_ Hconf]".
+    {  rewrite -(insert_insert _ PC _ (inl 0%Z)) Heq. iFrame "Hregs". iSplit;[iPureIntro|].
       - simpl. intros x. apply elem_of_gmap_dom. rewrite !dom_insert_L Hdom' list_to_set_difference. clear.
         pose proof (all_registers_s_correct x). set_solver.
       - iIntros (r HPC). rewrite /RegLocate. rewrite lookup_insert_ne//.
@@ -253,8 +246,8 @@ Section lse.
         rewrite Hdom'. clear -HPC n. pose proof (all_registers_s_correct r).
         rewrite list_to_set_difference. set_solver. }
     iApply (wp_wand with "Hconf").
-    iIntros (v). iIntros "Hcond". iApply "Hφ".
-    iIntros (Hhalted). iDestruct ("Hcond" $! Hhalted) as (r W'') "(?&?&%&?&?&?)".
+    iIntros (v). iIntros "Hcond'". iApply "Hφ".
+    iIntros (Hhalted). iDestruct ("Hcond'" $! Hhalted) as (r W'') "(?&?&%&?&?&?)".
     iExists _,_;iFrame.
     iPureIntro. eapply related_sts_a_priv_trans_world;eauto.
   Qed.
