theories/examples/world_changes.v
@@ -1,0 +1,32 @@
+From iris.algebra Require Import frac.
+From iris.proofmode Require Import tactics.
+Require Import Eqdep_dec List.
+From cap_machine Require Import rules logrel fundamental region_invariants_batch_uninitialized region_invariants_revocation region_invariants_static.
+From cap_machine Require Export iris_extra addr_reg_sample region_macros contiguous stack_macros_helpers.
+From cap_machine Require Import macros.
+
+(**
+   This file contains quality of life lemmas about world manipulations, for the
+   purpose of examples.
+ *)
+
+Section world.
+  Context {Σ:gFunctors} {memg:memG Σ} {regg:regG Σ}
+          {stsg : STSG Addr region_type Σ} {heapg : heapG Σ}
+          `{MonRef: MonRefG (leibnizO _) CapR_rtc Σ} {nainv: logrel_na_invs Σ}
+          `{MachineParameters}.
+
+  Notation STS := (leibnizO (STS_states * STS_rels)).
+  Notation STS_STD := (leibnizO (STS_std_states Addr region_type)).
+  Notation WORLD := (prodO STS_STD STS).
+  Implicit Types W : WORLD.
+
+
+  (* For example that use a dynamic type check to reinstate validity of a revoked world *)
+  Lemma region_open_acc W W1 l p g b e a :
+    ⊢ region W1 ∗ ([∗ list] a ∈ l, (∃ p φ, ⌜forall Wv, Persistent (φ Wv)⌝ ∗ ▷ monotemp_resources W φ a p ∗ rel a p φ) ∗ ⌜(std (revoke W)) !! a = Some Revoked⌝).
+
+
+
+
+End world.
